lang.v
@@ -106,10 +106,10 @@ Inductive expr_has_type : ty_ctx -> expr -> type -> Prop :=
 | ty_const_exch (g : ty_ctx) (t : type) : expr_has_type g exch ((Ref t) >> t >> t)
 (* General Expressions *)
 | ty_var (g : ty_ctx) (x : var) (t : type) (xfree : disj_vars (VarSet.singleton x) g)
-  : expr_has_type (join_double (judge x t) g xfree) x t
+  : expr_has_type (ctx_union (judge x t) g xfree) x t
 | ty_lam (g : ty_ctx) (x : var) (e : expr) (t1 t2 : type)
          (xfree : disj_vars (VarSet.singleton x) g)
-         (_ : expr_has_type (join_double (judge x t1) g xfree) e t2)
+         (_ : expr_has_type (ctx_union (judge x t1) g xfree) e t2)
   : expr_has_type g (lam x t1 e) (t1 >> t2)
 | ty_app (g : ty_ctx) (e1 e2 : expr) (t1 t2 : type)
          (_ : expr_has_type g e1 (t1 >> t2))
@@ -120,19 +120,19 @@ Inductive expr_has_type : ty_ctx -> expr -> type -> Prop :=
 Inductive config_has_type : ty_ctx -> config -> ty_ctx -> Prop :=
 | ty_config_par (g g1 g2 : ty_ctx) (c1 c2 : config)
                 (g_g1 : disj_vars g g1) (g_g2 : disj_vars g g2) (g1_g2 : disj_vars g1 g2)
-                (p1 : config_has_type (join_double g g1 g_g1) c1 g2)
-                (p2 : config_has_type (join_double g g2 g_g2) c2 g1)
-  : config_has_type g (c1 $$ c2) (join_double g1 g2 g1_g2)
+                (p1 : config_has_type (ctx_union g g1 g_g1) c1 g2)
+                (p2 : config_has_type (ctx_union g g2 g_g2) c2 g1)
+  : config_has_type g (c1 $$ c2) (ctx_union g1 g2 g1_g2)
 | ty_config_ref (g : ty_ctx) (x : var) (t : type) (v : val)
                 (disj_prf : disj_vars (VarSet.singleton x) g)
-                (vprf : expr_has_type (join_double (judge x (Ref t)) g disj_prf) v t)
+                (vprf : expr_has_type (ctx_union (judge x (Ref t)) g disj_prf) v t)
   : config_has_type g (x c= v) (judge x (Ref t))
 | ty_config_reserveplace (g g': ty_ctx) (c : config) (x : var)
                          (h : config_has_type g c g')
   : config_has_type g (x ** c) (restrict_ty_ctx g' x)
 | ty_config_threadval (g : ty_ctx) (x : var) (t : type) (e : expr)
                       (x_gfree : disj_vars (VarSet.singleton x) g)
-                      (h : expr_has_type (join_double (judge x t) g x_gfree) e t)
+                      (h : expr_has_type (ctx_union (judge x t) g x_gfree) e t)
   : config_has_type g (threadval x e) (judge x t)
 | ty_config_handledfut(g : ty_ctx) (x y : var) (t : type)
                       (x_not_y : ~(x = y))
@@ -151,6 +151,15 @@ Proof.
   intros C_Orig C_Final ty_prf cong_prf.
   destruct cong_prf.
   + inversion ty_prf.
+    clear g H H1 H2 c0 c3.
+    pose (disj_symmetry := disj_vars_sym g1 g2).
+    inversion disj_symmetry. clear H1.
+    pose (g2_g1 := H g1_g2).
+    pose (almost_goal := ty_config_par G g2 g1 c2 c1 g_g2 g_g1 g2_g1 p2 p1).
+    pose (needed_eql := ctx_union_sym g1 g2 g1_g2 g2_g1).
+    rewrite <- needed_eql in almost_goal.
+    assumption.
+
 
 (* Theorem SubjectReduction : (forall C1 C2 : config, forall G G' : ty_ctx, *)
 (*                             forall C1_Type : config_has_type G C1 G', *)
